thy/Iptables_Semantics/Firewall_Common.thy
@@ -1,5 +1,5 @@
 theory Firewall_Common
-imports Main Firewall_Common_Decision_State
+imports Main "../Simple_Firewall/Firewall_Common_Decision_State"
 begin
 
 section\<open>Firewall Basic Syntax\<close>
@@ -22,7 +22,8 @@ definition MatchOr :: "'a match_expr \<Rightarrow> 'a match_expr \<Rightarrow> '
 
 datatype 'a rule = Rule (get_match: "'a match_expr") (get_action: action)
 
-lemma rules_singleton_rev_E: "[Rule m a] = rs\<^sub>1 @ rs\<^sub>2 \<Longrightarrow> (rs\<^sub>1 = [Rule m a] \<Longrightarrow> rs\<^sub>2 = [] \<Longrightarrow> P m a) \<Longrightarrow> (rs\<^sub>1 = [] \<Longrightarrow> rs\<^sub>2 = [Rule m a] \<Longrightarrow> P m a) \<Longrightarrow> P m a"
+lemma rules_singleton_rev_E:
+  "[Rule m a] = rs\<^sub>1 @ rs\<^sub>2 \<Longrightarrow> (rs\<^sub>1 = [Rule m a] \<Longrightarrow> rs\<^sub>2 = [] \<Longrightarrow> P m a) \<Longrightarrow> (rs\<^sub>1 = [] \<Longrightarrow> rs\<^sub>2 = [Rule m a] \<Longrightarrow> P m a) \<Longrightarrow> P m a"
 by (cases rs\<^sub>1) auto
 
 
