thy/Iptables_Semantics/Primitive_Matchers/Common_Primitive_Syntax.thy
@@ -1,6 +1,6 @@
 theory Common_Primitive_Syntax
 imports "../Datatype_Selectors"
-        IpAddresses Iface Protocol Ports Simple_Packet Conntrack_State
+        IpAddresses Iface L4_Protocol_Flags Ports Tagged_Packet Conntrack_State
 begin
 
 section\<open>Primitive Matchers: Interfaces, IP Space, Layer 4 Ports Matcher\<close>
