thy/Iptables_Semantics/Primitive_Matchers/Common_Primitive_toString.thy
@@ -1,6 +1,6 @@
 theory Common_Primitive_toString
 imports 
-        "../Common/Lib_toString"
+        "../../Simple_Firewall/Common/Lib_toString"
         "../../IP_Addresses/IP_Address_toString"
         Common_Primitive_Matcher
 begin
