thy/Iptables_Semantics/Primitive_Matchers/L4_Protocol_Flags.thy
@@ -1,94 +1,8 @@
-theory Protocol
-imports "../Common/Negation_Type" "../Common/Lib_toString" "~~/src/HOL/Word/Word"
+theory L4_Protocol_Flags
+imports "../../Simple_Firewall/L4_Protocol"
 begin
 
-section\<open>Protocols\<close>
-
-type_synonym primitive_protocol = "8 word"
-
-definition "ICMP \<equiv> 1 :: 8 word"
-definition "TCP \<equiv> 6 :: 8 word"
-definition "UDP \<equiv> 17 :: 8 word"
-definition "SCTP \<equiv> 132  :: 8 word"
-(* turn http://www.iana.org/assignments/protocol-numbers/protocol-numbers.xhtml into a separate file or so? *)
-
-datatype protocol = ProtoAny | Proto "primitive_protocol" (*probably negation_type?*)
-
-(*TODO add negation type. Conjunction is still easy since we don't have wildcards
-  E.g. TCP \<and> \<not> UDP \<longleftrightarrow> TCP
-       TCP \<and> \<not> TCP \<longleftrightarrow> False
-       TCP \<and> UDP \<longleftrightarrow> TCP = UDP
-*)
-
-fun match_proto :: "protocol \<Rightarrow> primitive_protocol \<Rightarrow> bool" where
-  "match_proto ProtoAny _ \<longleftrightarrow> True" |
-  "match_proto (Proto (p)) p_p \<longleftrightarrow> p_p = p"
-
-  fun simple_proto_conjunct :: "protocol \<Rightarrow> protocol \<Rightarrow> protocol option" where
-    "simple_proto_conjunct ProtoAny proto = Some proto" |
-    "simple_proto_conjunct proto ProtoAny = Some proto" |
-    "simple_proto_conjunct (Proto p1) (Proto p2) = (if p1 = p2 then Some (Proto p1) else None)"
-  lemma simple_proto_conjunct_asimp[simp]: "simple_proto_conjunct proto ProtoAny = Some proto"
-    by(cases proto) simp_all
-
-  lemma simple_proto_conjunct_correct: "match_proto p1 pkt \<and> match_proto p2 pkt \<longleftrightarrow> 
-    (case simple_proto_conjunct p1 p2 of None \<Rightarrow> False | Some proto \<Rightarrow> match_proto proto pkt)"
-    apply(cases p1)
-     apply(simp_all)
-    apply(rename_tac pp1)
-    apply(cases p2)
-     apply(simp_all)
-    done
-
-
-  lemma simple_proto_conjunct_Some: "simple_proto_conjunct p1 p2 = Some proto \<Longrightarrow> 
-    match_proto proto pkt \<longleftrightarrow> match_proto p1 pkt \<and> match_proto p2 pkt"
-    using simple_proto_conjunct_correct by simp
-  lemma simple_proto_conjunct_None: "simple_proto_conjunct p1 p2 = None \<Longrightarrow> 
-    \<not> (match_proto p1 pkt \<and> match_proto p2 pkt)"
-    using simple_proto_conjunct_correct by simp
-
-
-  text\<open>Originally, there was a @{typ nat} in the protocol definition, allowing infinitly many protocols 
-        This was intended behavior. We want to prevent things such as @{term "\<not>TCP = UDP"}.
-        So be careful with what you prove...\<close>
-  lemma primitive_protocol_Ex_neq: "p = Proto pi \<Longrightarrow> \<exists>p'. p' \<noteq> pi" 
-  proof
-  	show "pi + 1 \<noteq> pi" by simp
-  qed
-  lemma protocol_Ex_neq: "\<exists>p'. Proto p' \<noteq> p"
-    by(cases p) (simp_all add: primitive_protocol_Ex_neq)
-
-section\<open>TCP flags\<close>
-  datatype tcp_flag = TCP_SYN | TCP_ACK | TCP_FIN | TCP_RST | TCP_URG | TCP_PSH (*| TCP_ALL | TCP_NONE*)
-
-  lemma UNIV_tcp_flag: "UNIV = {TCP_SYN, TCP_ACK, TCP_FIN, TCP_RST, TCP_URG, TCP_PSH}" using tcp_flag.exhaust by auto 
-  instance tcp_flag :: finite
-  proof
-    from UNIV_tcp_flag show "finite (UNIV:: tcp_flag set)" using finite.simps by auto 
-  qed
-  instantiation "tcp_flag" :: enum
-  begin
-    definition "enum_tcp_flag = [TCP_SYN, TCP_ACK, TCP_FIN, TCP_RST, TCP_URG, TCP_PSH]"
-  
-    definition "enum_all_tcp_flag P \<longleftrightarrow> P TCP_SYN \<and> P TCP_ACK \<and> P TCP_FIN \<and> P TCP_RST \<and> P TCP_URG \<and> P TCP_PSH"
-    
-    definition "enum_ex_tcp_flag P \<longleftrightarrow> P TCP_SYN \<or> P TCP_ACK \<or> P TCP_FIN \<or> P TCP_RST \<or> P TCP_URG \<or> P TCP_PSH"
-  instance proof
-    show "UNIV = set (enum_class.enum :: tcp_flag list)"
-      by(simp add: UNIV_tcp_flag enum_tcp_flag_def)
-    next
-    show "distinct (enum_class.enum :: tcp_flag list)"
-      by(simp add: enum_tcp_flag_def)
-    next
-    show "\<And>P. (enum_class.enum_all :: (tcp_flag \<Rightarrow> bool) \<Rightarrow> bool) P = Ball UNIV P"
-      by(simp add: UNIV_tcp_flag enum_all_tcp_flag_def)
-    next
-    show "\<And>P. (enum_class.enum_ex :: (tcp_flag \<Rightarrow> bool) \<Rightarrow> bool) P = Bex UNIV P"
-      by(simp add: UNIV_tcp_flag enum_ex_tcp_flag_def)
-  qed
-  end
-  
+section\<open>Matching TCP Flags\<close>
   (*man iptables-extensions, [!] --tcp-flags mask comp*)
   datatype ipt_tcp_flags = TCP_Flags "tcp_flag set" --"mask"
                                      "tcp_flag set" --"comp"
@@ -218,21 +132,4 @@ section\<open>TCP flags\<close>
      done
   end
   declare ipt_tcp_flags_equal.simps[simp del]
-
-
-  fun tcp_flag_toString :: "tcp_flag \<Rightarrow> string" where
-    "tcp_flag_toString TCP_SYN = ''TCP_SYN''" |
-    "tcp_flag_toString TCP_ACK = ''TCP_ACK''" |
-    "tcp_flag_toString TCP_FIN = ''TCP_FIN''" |
-    "tcp_flag_toString TCP_RST = ''TCP_RST''" |
-    "tcp_flag_toString TCP_URG = ''TCP_URG''" |
-    "tcp_flag_toString TCP_PSH = ''TCP_PSH''"
-
-
-  definition ipt_tcp_flags_toString :: "tcp_flag set \<Rightarrow> char list" where
-    "ipt_tcp_flags_toString flags \<equiv> list_toString tcp_flag_toString (enum_set_to_list flags)"
-
-  lemma "ipt_tcp_flags_toString {TCP_SYN,TCP_SYN,TCP_ACK} = ''[TCP_SYN, TCP_ACK]''" by eval
-
-
 end
