thy/Iptables_Semantics/Primitive_Matchers/Tagged_Packet.thy
@@ -1,0 +1,50 @@
+theory Tagged_Packet
+imports "../../Simple_Firewall/Simple_Packet" Conntrack_State
+begin
+
+section\<open>Tagged Simple Packet\<close>
+  text\<open>Packet constants are prefixed with @{text p}\<close>
+
+  text\<open>A packet tagged with the following phantom fields:
+             conntrack connection state\<close>
+
+  text\<open>The idea to tag the connection state into the packet is sound.
+       See @{file "../Semantics_Stateful.thy"}\<close>
+
+  record (overloaded) 'i tagged_packet = "'i::len simple_packet" +
+                         p_tag_ctstate :: ctstate
+
+
+  value "\<lparr> 
+          p_iiface = ''eth1'', p_oiface = '''', 
+          p_src = 0, p_dst = 0, 
+          p_proto = TCP, p_sport = 0, p_dport = 0, 
+          p_tcp_flags = {TCP_SYN},
+          p_payload = ''arbitrary payload'',
+          p_tag_ctstate = CT_New
+         \<rparr>:: 32 tagged_packet"
+
+  definition simple_packet_tag
+    :: "ctstate \<Rightarrow> ('i::len, 'a) simple_packet_scheme \<Rightarrow> ('i::len, 'a) tagged_packet_scheme" where
+    "simple_packet_tag ct_state p \<equiv>
+      \<lparr>p_iiface = p_iiface p, p_oiface = p_oiface p, p_src = p_src p, p_dst = p_dst p, p_proto = p_proto p, 
+       p_sport = p_sport p, p_dport = p_dport p, p_tcp_flags = p_tcp_flags p, 
+       p_payload = p_payload p,
+       p_tag_ctstate = ct_state,
+       \<dots> = simple_packet.more p\<rparr>"
+
+  definition tagged_packet_untag
+    :: "('i::len, 'a) tagged_packet_scheme \<Rightarrow> ('i::len, 'a) simple_packet_scheme" where
+    "tagged_packet_untag p \<equiv>
+      \<lparr>p_iiface = p_iiface p, p_oiface = p_oiface p, p_src = p_src p, p_dst = p_dst p, p_proto = p_proto p, 
+       p_sport = p_sport p, p_dport = p_dport p, p_tcp_flags = p_tcp_flags p, 
+       p_payload = p_payload p,
+       \<dots> = tagged_packet.more p\<rparr>"
+
+  lemma "tagged_packet_untag (simple_packet_tag ct_state p) = p"
+        "simple_packet_tag ct_state (tagged_packet_untag p) = p\<lparr>p_tag_ctstate := ct_state\<rparr>"
+    apply(case_tac [!] p)
+     by(simp add: tagged_packet_untag_def simple_packet_tag_def)+
+    
+
+end
