thy/Simple_Firewall/SimpleFw_Semantics.thy
@@ -1,78 +1,10 @@
 theory SimpleFw_Semantics
-imports Main "../Common/Negation_Type"
-  "../Firewall_Common_Decision_State"
-  "../Primitive_Matchers/IpAddresses"
-  "../Primitive_Matchers/Iface"
-  "../Primitive_Matchers/Protocol"
-  "../Primitive_Matchers/Simple_Packet"
+imports SimpleFw_Syntax
+  "../Iptables_Semantics/Common/Negation_Type"
+  "../Iptables_Semantics/Primitive_Matchers/IpAddresses"
   "../../IP_Addresses/Hs_Compat"
 begin
 
-
-section\<open>Simple Firewall Syntax (for IP addresses of arbitrary length)\<close>
-
-
-  datatype simple_action = Accept | Drop
-  
-  text\<open>Simple match expressions do not allow negated expressions.
-        However, Most match expressions can still be transformed into simple match expressions.
-        
-        A negated IP address range can be represented as a set of non-negated IP ranges.
-        For example @{text "!8 = {0..7} \<union> {8 .. ipv4max}"}.
-        Using CIDR notation (i.e. the @{text "a.b.c.d/n"} notation), we can represent negated IP
-        ranges as a set of non-negated IP ranges with only fair blowup.
-        Another handy result is that the conjunction of two IP ranges in CIDR notation is 
-        either the smaller of the two ranges or the empty set.
-        An empty IP range cannot be represented.
-        If one wants to represent the empty range, then the complete rule needs to be removed.
-
-        The same holds for layer 4 ports.
-        In addition, there exists an empty port range, e.g. @{text "(1,0)"}.
-        The conjunction of two port ranges is again just one port range.
-        
-        But negation of interfaces is not supported. Since interfaces support a wildcard character,
-        transforming a negated interface would either result in an infeasible blowup or requires
-        knowledge about the existing interfaces (e.g. there only is eth0, eth1, wlan3, and vbox42)
-        An empirical test shows that negated interfaces do not occur in our data sets.
-        Negated interfaces can also be considered bad style: What is !eth0? Everything that is
-        not eth0, experience shows that interfaces may come up randomly, in particular in combination 
-        with virtual machines, so !eth0 might not be the desired match.
-        At the moment, if an negated interface occurs which prevents translation to a simple match,
-        we recommend to abstract the negated interface to unknown and remove it (upper or lower closure
-        rule set) before translating to a simple match.
-        The same discussion holds for negated protocols.
-
-        Noteworthy, simple match expressions are both expressive and support conjunction:
-        @{text "simple-match1 \<and> simple-match2 = simple-match3"}
-\<close>
-        (*It took very long to design the simple match such that it can represent everything we need
-        and that you can calculate with it. Disjunction is easy: just have two consecutive rules with the same action.
-        Conjunction was a tough fight! It is needed to translate:
-        common_primitive_match_to_simple_match (MatchAny e1 e2) =
-          simple_match_and (common_primitive_match_to_simple_match e1) (common_primitive_match_to_simple_match e2)
-        This is key to translate common_primitive_match to simple_match
-
-        It may seem a simple enhancement to support iiface :: "iface negation_type", but then you
-        can no longer for the conjunction of two simple_matches.
-        *)
-
-  record (overloaded) 'i simple_match =
-    iiface :: "iface" --"in-interface"
-      (*we cannot (and don't want to, c.f. git history) express negated interfaces*)
-      (*We could also drop interface wildcard support and try negated interfaces again \<dots>*)
-    oiface :: "iface" --"out-interface"
-    src :: "('i::len word \<times> nat) " --"source IP address"
-    dst :: "('i::len word \<times> nat) " --"destination"
-    proto :: "protocol"
-    sports :: "(16 word \<times> 16 word)" --"source-port first:last"
-    dports :: "(16 word \<times> 16 word)" --"destination-port first:last"
-
-  
-  context
-    notes [[typedef_overloaded]]
-  begin
-    datatype 'i simple_rule = SimpleRule (match_sel: "'i simple_match") (action_sel: simple_action)
-  end
 
 subsection\<open>Simple Firewall Semantics\<close>
 
@@ -412,7 +344,7 @@ begin
 
   lemma "simple_fw [SimpleRule example_simple_match1 simple_action.Drop]
     \<lparr>p_iiface = '''', p_oiface = '''',  p_src = (1::ipv4addr), p_dst = 2, p_proto = TCP, p_sport = 8,
-     p_dport = 9, p_tcp_flags = {}, p_payload = '''', p_tag_ctstate = CT_New\<rparr> =
+     p_dport = 9, p_tcp_flags = {}, p_payload = ''''\<rparr> =
       Decision FinalDeny" by eval
 
   private definition "example_simple_match2 \<equiv> example_simple_match1\<lparr> proto := ProtoAny \<rparr>"
